trillium/program_logic/traces.v
@@ -404,3 +404,4 @@ Section simulation.
   Qed.
 
 End simulation.
+  
